theories/simulations/sim_hmod/HPSimFacts.v
@@ -7,11 +7,11 @@ Section HPSIM_ADEQUACY.
   Context `{Σ : GRA}.
   Notation iProp := (iProp Σ).
 
+  Variable contextual: contextuality.
   Variable fl_src : alist string (Any.t -> itree hmodE Any.t).
   Variable fl_tgt : alist string (Any.t -> itree hmodE Any.t).
   Variable Ist : nat -> alist key Any.t -> alist key Any.t -> iProp.
   Variable my_tid : nat.
-  Variable is_closed: bool.
 
   (*** Used only in hpsim_adequacy. ***)
   Lemma own_upd_in_middle mr_src mr_tgt ctx fmr fmr0
@@ -96,7 +96,7 @@ Section HPSIM_ADEQUACY.
       (NODUPT : List.NoDup (List.map fst st_tgt)) :
     interp_inv ctx (nths, Any.pair (alist_encode st_src) mr_src↑, Any.pair (alist_encode st_tgt) mr_tgt↑).
 
-  (* Now, adequacy requires 'is_closed = true'*)
+  (* Adequacy requires 'contextual = closed'*)
   Lemma hpsim_adequacy
       (NODUPFS : List.NoDup (List.map fst fl_src))
       (NODUPFT : List.NoDup (List.map fst fl_tgt))
@@ -109,7 +109,7 @@ Section HPSIM_ADEQUACY.
       (ctx0 ctx : list Σ) (mr_src mr_tgt fmr : Σ)
       (CTXLE : @le_mine Σ eq my_tid ctx0 ctx)
       (TID : my_tid < List.length ctx0)
-      (SIM : hpsim_body fl_src fl_tgt Ist my_tid true ps pt nths (st_src, itr_src) (st_tgt, itr_tgt) fmr)
+      (SIM : hpsim_body closed fl_src fl_tgt Ist my_tid ps pt nths (st_src, itr_src) (st_tgt, itr_tgt) fmr)
       (WF : ✓ mr_src)
       (FMR : Own mr_src ⊢ |==> Own ((ctx_sem ctx) ⋅ fmr ⋅ mr_tgt)) :
     @sim_itree fl_src0 fl_tgt0 Σ ε interp_inv eq my_tid ctx0 ps pt ctx nths
